thys/MFOTL_Monitor/Trace.thy
@@ -4,7 +4,9 @@ theory Trace
 begin
 (*>*)
 
-section \<open>Infinite Traces\<close>
+section \<open>Traces and trace prefixes\<close>
+
+subsection \<open>Infinite traces\<close>
 
 coinductive ssorted :: "'a :: linorder stream \<Rightarrow> bool" where
   "shd s \<le> shd (stl s) \<Longrightarrow> ssorted (stl s) \<Longrightarrow> ssorted s"
@@ -37,21 +39,58 @@ lemma ssorted_monoI: "\<forall>i j. i \<le> j \<longrightarrow> s !! i \<le> s !
 lemma ssorted_iff_mono: "ssorted s \<longleftrightarrow> (\<forall>i j. i \<le> j \<longrightarrow> s !! i \<le> s !! j)"
   using ssorted_monoI ssorted_monoD by metis
 
-definition "sincreasing s = (\<forall>i. \<exists>j>i. s !! i < s !! j)"
+lemma ssorted_iff_le_Suc: "ssorted s \<longleftrightarrow> (\<forall>i. s !! i \<le> s !! Suc i)"
+  using mono_iff_le_Suc[of "snth s"] by (simp add: mono_def ssorted_iff_mono)
 
-lemma sincreasing_siterate[simp]:
+definition "sincreasing s = (\<forall>x. \<exists>i. x < s !! i)"
+
+lemma sincreasingI: "(\<And>x. \<exists>i. x < s !! i) \<Longrightarrow> sincreasing s"
+  by (simp add: sincreasing_def)
+
+lemma sincreasing_grD:
+  fixes x :: "'a :: semilattice_sup"
+  assumes "sincreasing s"
+  shows "\<exists>j>i. x < s !! j"
+proof -
+  let ?A = "insert x {s !! n | n. n \<le> i}"
+  from assms obtain j where *: "Sup_fin ?A < s !! j"
+    by (auto simp: sincreasing_def)
+  then have "x < s !! j"
+    by (rule order.strict_trans1[rotated]) (auto intro: Sup_fin.coboundedI)
+  moreover have "i < j"
+  proof (rule ccontr)
+    assume "\<not> i < j"
+    then have "s !! j \<in> ?A" by (auto simp: not_less)
+    then have "s !! j \<le> Sup_fin ?A"
+      by (auto intro: Sup_fin.coboundedI)
+    with * show False by simp
+  qed
+  ultimately show ?thesis by blast
+qed
+
+lemma sincreasing_siterate_nat[simp]:
+  fixes n :: nat
   assumes "(\<And>n. n < f n)"
   shows "sincreasing (siterate f n)"
 unfolding sincreasing_def proof
-  fix i
-  show "\<exists>j>i. siterate f n !! i < siterate f n !! j" (is "\<exists>j. ?P n i j")
-  proof (induct i arbitrary: n)
-    case (Suc i)
-    from Suc[of "f n"] obtain j where "?P (f n) i j" by blast
-    then show ?case
-      by (intro exI[of _ "Suc j"]) auto
-  qed (auto intro!: exI[of _ "Suc 0"] assms)
+  fix x
+  show "\<exists>i. x < siterate f n !! i"
+  proof (induction x)
+    case 0
+    have "0 < siterate f n !! 1"
+      using order.strict_trans1[OF le0 assms] by simp
+    then show ?case ..
+  next
+    case (Suc x)
+    then obtain i where "x < siterate f n !! i" ..
+    then have "Suc x < siterate f n !! Suc i"
+      using order.strict_trans1[OF _ assms] by (simp del: snth.simps)
+    then show ?case ..
+  qed
 qed
+
+lemma sincreasing_stl: "sincreasing s \<Longrightarrow> sincreasing (stl s)" for s :: "'a :: semilattice_sup stream"
+  by (auto 0 4 simp: gr0_conv_Suc intro!: sincreasingI dest: sincreasing_grD[of s 0])
 
 typedef 'a trace = "{s :: ('a set \<times> nat) stream. ssorted (smap snd s) \<and> sincreasing (smap snd s)}"
   by (intro exI[of _ "smap (\<lambda>i. ({}, i)) nats"])
@@ -64,23 +103,17 @@ lift_definition \<Gamma> :: "'a trace \<Rightarrow> nat \<Rightarrow> 'a set" is
 lift_definition \<tau> :: "'a trace \<Rightarrow> nat \<Rightarrow> nat" is
   "\<lambda>s i. snd (s !! i)" .
 
+lemma stream_eq_iff: "s = s' \<longleftrightarrow> (\<forall>n. s !! n = s' !! n)"
+  by (metis stream.map_cong0 stream_smap_nats)
+
+lemma trace_eqI: "(\<And>i. \<Gamma> \<sigma> i = \<Gamma> \<sigma>' i) \<Longrightarrow> (\<And>i. \<tau> \<sigma> i = \<tau> \<sigma>' i) \<Longrightarrow> \<sigma> = \<sigma>'"
+  by transfer (auto simp: stream_eq_iff intro!: prod_eqI)
+
 lemma \<tau>_mono[simp]: "i \<le> j \<Longrightarrow> \<tau> s i \<le> \<tau> s j"
   by transfer (auto simp: ssorted_iff_mono)
 
 lemma ex_le_\<tau>: "\<exists>j\<ge>i. x \<le> \<tau> s j"
-proof (transfer fixing: i x)
-  fix s :: "('a set \<times> nat) stream"
-  presume sincreasing: "sincreasing (smap snd s)"
-  show "\<exists>j\<ge>i. x \<le> snd (s !! j)" proof (induction x)
-    case 0
-    show ?case by auto
-  next
-    case (Suc x)
-    then show ?case
-      using sincreasing unfolding sincreasing_def
-      by (metis Suc_le_eq le_less_trans less_imp_le_nat snth_smap)
-  qed
-qed simp
+  by (transfer fixing: i x) (auto dest!: sincreasing_grD[of _ i x] less_imp_le)
 
 lemma le_\<tau>_less: "\<tau> \<sigma> i \<le> \<tau> \<sigma> j \<Longrightarrow> j < i \<Longrightarrow> \<tau> \<sigma> i = \<tau> \<sigma> j"
   by (simp add: antisym)
@@ -110,12 +143,16 @@ lemma map_\<Gamma>_cong: "\<sigma>\<^sub>1 = \<sigma>\<^sub>2 \<Longrightarrow> 
   by transfer (auto intro!: stream.map_cong)
 
 
-section \<open>Finite Trace Prefixes\<close>
+subsection \<open>Finite trace prefixes\<close>
 
 typedef 'a prefix = "{p :: ('a set \<times> nat) list. sorted (map snd p)}"
   by (auto intro!: exI[of _ "[]"])
 
 setup_lifting type_definition_prefix
+
+lift_definition pmap_\<Gamma> :: "('a set \<Rightarrow> 'b set) \<Rightarrow> 'a prefix \<Rightarrow> 'b prefix" is
+  "\<lambda>f. map (\<lambda>(x, i). (f x, i))"
+  by (simp add: split_beta comp_def)
 
 lift_definition last_ts :: "'a prefix \<Rightarrow> nat" is
   "\<lambda>p. (case p of [] \<Rightarrow> 0 | _ \<Rightarrow> snd (last p))" .
@@ -172,6 +209,9 @@ lemma prefix_of_pnil[simp]: "prefix_of pnil \<sigma>"
 lemma plen_pnil[simp]: "plen pnil = 0"
   by transfer auto
 
+lemma prefix_of_pmap_\<Gamma>[simp]: "prefix_of \<pi> \<sigma> \<Longrightarrow> prefix_of (pmap_\<Gamma> f \<pi>) (map_\<Gamma> f \<sigma>)"
+  by transfer auto
+
 lemma plen_mono: "\<pi> \<le> \<pi>' \<Longrightarrow> plen \<pi> \<le> plen \<pi>'"
   by transfer auto
 
@@ -203,6 +243,28 @@ lemma pdrop_0[simp]: "pdrop 0 \<pi> = \<pi>"
 lemma prefix_of_antimono: "\<pi> \<le> \<pi>' \<Longrightarrow> prefix_of \<pi>' s \<Longrightarrow> prefix_of \<pi> s"
   by transfer (auto simp del: stake_add simp add: stake_add[symmetric])
 
+lemma prefix_of_imp_linear: "prefix_of \<pi> \<sigma> \<Longrightarrow> prefix_of \<pi>' \<sigma> \<Longrightarrow> \<pi> \<le> \<pi>' \<or> \<pi>' \<le> \<pi>"
+proof transfer
+  fix \<pi> \<pi>' and \<sigma> :: "('a set \<times> nat) stream"
+  assume assms: "stake (length \<pi>) \<sigma> = \<pi>" "stake (length \<pi>') \<sigma> = \<pi>'"
+  show "(\<exists>r. \<pi>' = \<pi> @ r) \<or> (\<exists>r. \<pi> = \<pi>' @ r)"
+  proof (cases "length \<pi>" "length \<pi>'" rule: le_cases)
+    case le
+    then have "\<pi>' = take (length \<pi>) \<pi>' @ drop (length \<pi>) \<pi>'"
+      by simp
+    moreover have "take (length \<pi>) \<pi>' = \<pi>"
+      using assms le by (metis min.absorb1 take_stake)
+    ultimately show ?thesis by auto
+  next
+    case ge
+    then have "\<pi> = take (length \<pi>') \<pi> @ drop (length \<pi>') \<pi>"
+      by simp
+    moreover have "take (length \<pi>') \<pi> = \<pi>'"
+      using assms ge by (metis min.absorb1 take_stake)
+    ultimately show ?thesis by auto
+  qed
+qed
+
 lemma ex_prefix_of: "\<exists>s. prefix_of p s"
 proof (transfer, intro bexI CollectI conjI)
   fix p :: "('a set \<times> nat) list"
@@ -214,19 +276,12 @@ proof (transfer, intro bexI CollectI conjI)
     by (cases p) (auto simp: last_conv_nth nth_Cons')
   with * show "ssorted (smap snd ?\<sigma>)"
     by (force simp: ssorted_iff_mono sorted_iff_nth_mono shift_snth)
-  show "sincreasing (smap snd ?\<sigma>)" unfolding sincreasing_def
-  proof (rule allI)
-    fix i
-    show "\<exists>j > i.  smap snd ?\<sigma> !! i < smap snd ?\<sigma> !! j"
-    proof (cases "i < length p")
-      case True
-      with le_last[of i] show ?thesis
-        by (auto intro!: exI[of _ "Suc (length p)"])
-    next
-      case False
-      then show ?thesis
-        by (auto simp: neq_Nil_conv intro!: exI[of _ "Suc i"])
-    qed
+  show "sincreasing (smap snd ?\<sigma>)"
+  proof (rule sincreasingI)
+    fix x
+    have "x < smap snd ?\<sigma> !! Suc (length p + x)"
+      by simp (metis Suc_pred add.commute diff_Suc_Suc length_greater_0_conv less_add_Suc1 less_diff_conv)
+    then show "\<exists>i. x < smap snd ?\<sigma> !! i" ..
   qed
 qed
 
@@ -237,14 +292,16 @@ lemma \<Gamma>_prefix_conv: "prefix_of p s \<Longrightarrow> prefix_of p s' \<Lo
   by transfer (simp add: stake_nth[symmetric])
 
 lemma sincreasing_sdrop:
+  fixes s :: "('a :: semilattice_sup) stream"
   assumes "sincreasing s"
   shows "sincreasing (sdrop n s)"
-proof (unfold sincreasing_def; safe)
-  fix i
-  from assms obtain j where "n + i < j" "s !! (n + i) < s !! j"
-    unfolding sincreasing_def by auto
-  then show "\<exists>j>i. sdrop n s !! i < sdrop n s !! j"
-    by (auto simp: sdrop_snth intro!: exI[of _ "j - n"])
+proof (rule sincreasingI)
+  fix x
+  obtain i where "n < i" and "x < s !! i"
+    using sincreasing_grD[OF assms] by blast
+  then have "x < sdrop n s !! (i - n)"
+    by (simp add: sdrop_snth)
+  then show "\<exists>i. x < sdrop n s !! i" ..
 qed
 
 lemma ssorted_shift:
@@ -270,23 +327,15 @@ next
 qed
 
 lemma sincreasing_shift:
-  assumes "ssorted (xs @- s)" "sincreasing s"
+  assumes "sincreasing s"
   shows "sincreasing (xs @- s)"
-proof (unfold sincreasing_def; safe)
-  fix i
-  show "\<exists>j>i. (xs @- s) !! i < (xs @- s) !! j"
-  proof (cases "i < length xs")
-    case True
-    with assms(1) have "xs ! i \<le> shd s" unfolding ssorted_shift by (auto simp: shd_sset)
-    also obtain j where "\<dots> < s !! j"
-      using assms(2) by (auto simp: sincreasing_def dest: spec[of _ 0])
-    finally show ?thesis using True by (auto intro!: exI[of _ "j + length xs"])
-  next
-    case False
-    then obtain j where "i - length xs < j" "s !! (i - length xs) < s !! j"
-      using assms(2) by (auto simp: sincreasing_def)
-    then show ?thesis using False by (auto simp: not_less intro!: exI[of _ "j + length xs"])
-  qed
+proof (rule sincreasingI)
+  fix x
+  from assms obtain i where "x < s !! i"
+    unfolding sincreasing_def by blast
+  then have "x < (xs @- s) !! (length xs + i)"
+    by simp
+  then show "\<exists>i. x < (xs @- s) !! i" ..
 qed
 
 lift_definition replace_prefix :: "'a prefix \<Rightarrow> 'a trace \<Rightarrow> 'a trace" is
@@ -294,6 +343,49 @@ lift_definition replace_prefix :: "'a prefix \<Rightarrow> 'a trace \<Rightarrow
      \<pi> @- sdrop (length \<pi>) \<sigma> else smap (\<lambda>i. ({}, i)) nats"
   by (auto split: if_splits simp: stream.map_comp stream.map_ident sdrop_smap[symmetric]
     simp del: sdrop_smap intro!: sincreasing_shift sincreasing_sdrop cong: stream.map_cong)
+
+lemma prefix_of_replace_prefix:
+  "prefix_of (pmap_\<Gamma> f \<pi>) \<sigma> \<Longrightarrow> prefix_of \<pi> (replace_prefix \<pi> \<sigma>)"
+proof (transfer; safe; goal_cases)
+  case (1 f \<pi> \<sigma>)
+  then show ?case
+    by (subst (asm) (2) stake_sdrop[symmetric, of _ "length \<pi>"])
+      (auto 0 3 simp: ssorted_shift split_beta o_def stake_shift sdrop_smap[symmetric]
+        ssorted_sdrop not_le simp del: sdrop_smap)
+qed
+
+lemma map_\<Gamma>_replace_prefix:
+  "\<forall>x. f (f x) = f x \<Longrightarrow> prefix_of (pmap_\<Gamma> f \<pi>) \<sigma> \<Longrightarrow> map_\<Gamma> f (replace_prefix \<pi> \<sigma>) = map_\<Gamma> f \<sigma>"
+proof (transfer; safe; goal_cases)
+  case (1 f \<pi> \<sigma>)
+  then show ?case
+    by (subst (asm) (2) stake_sdrop[symmetric, of \<sigma> "length \<pi>"],
+        subst (3) stake_sdrop[symmetric, of \<sigma> "length \<pi>"])
+      (auto simp: ssorted_shift split_beta o_def stake_shift sdrop_smap[symmetric] ssorted_sdrop
+        not_le simp del: sdrop_smap cong: map_cong)
+qed
+
+lemma prefix_of_pmap_\<Gamma>_D:
+  assumes "prefix_of (pmap_\<Gamma> f \<pi>) \<sigma>"
+  shows "\<exists>\<sigma>'. prefix_of \<pi> \<sigma>' \<and> prefix_of (pmap_\<Gamma> f \<pi>) (map_\<Gamma> f \<sigma>')"
+proof -
+  from assms(1) obtain \<sigma>' where 1: "prefix_of \<pi> \<sigma>'"
+    using ex_prefix_of by blast
+  then have "prefix_of (pmap_\<Gamma> f \<pi>) (map_\<Gamma> f \<sigma>')"
+    by transfer simp
+  with 1 show ?thesis by blast
+qed
+
+lemma prefix_of_map_\<Gamma>_D:
+  assumes "prefix_of \<pi>' (map_\<Gamma> f \<sigma>)"
+  shows "\<exists>\<pi>''. \<pi>' = pmap_\<Gamma> f \<pi>'' \<and> prefix_of \<pi>'' \<sigma>"
+  using assms
+  by transfer (auto intro!: exI[of _ "stake (length _) _"] elim: sym dest: sorted_stake)
+
+lift_definition pts :: "'a prefix \<Rightarrow> nat list" is "map snd" .
+
+lemma pts_pmap_\<Gamma>[simp]: "pts (pmap_\<Gamma> f \<pi>) = pts \<pi>"
+  by (transfer fixing: f) (simp add: split_beta)
 
 (*<*)
 end
